Core/ProgramRules.v
@@ -3,6 +3,7 @@ From LHL.Core Require Import
   Specs
   Traces
   Logic
+  LogicPaco
   LogicFacts
   ProgramFacts.
 
@@ -14,78 +15,6 @@ From LHL.Util Require Import
   Tactics.
 
 From Paco Require Import paco.
-
-Inductive paco_safeF {E F A} {VE : Spec E} {VF : Spec F} i (R G : Relt VE VF) (Q : Post VE VF A) (rec : Relt VE VF -> Prog E A -> Prop) : Relt VE VF -> Prog E A -> Prop :=
-| SafeReturn v P :
-    P ==> Q v ->
-    paco_safeF i R G Q rec P (Return v)
-| SafeBind A (P : Relt VE VF) QI QR (m : E A) k :
-    Stable R QI ->
-    Stable R QR ->
-    Commit i G P (CallEv m) QI ->
-    (forall v,
-      Commit i G (P ->> QI) (RetEv m v) (QR v) /\
-      rec (P ->> QI ->> QR v) (k v)) ->
-    paco_safeF i R G Q rec P (Bind m k)
-| SafeNoOp (P : Relt VE VF) QS C :
-    Stable R QS ->
-    SilentStep i G P QS ->
-    rec (P ->> QS) C ->
-    paco_safeF i R G Q rec P (NoOp C)
-.
-
-Definition paco_safe {E F A} {VE : Spec E} {VF : Spec F} i (R G P : Relt VE VF) (C : Prog E A) (Q : Post VE VF A) : Prop := paco2 (paco_safeF i R G Q) bot2 P C.
-
-Lemma safe_monotone {E F A} {VE : Spec E} {VF : Spec F} (i : ThreadName) (R G : Relt VE VF) (Q : Post VE VF A) :
-  monotone2 (paco_safeF i R G Q).
-unfold monotone2. intros.
-destruct IN.
-econstructor. easy.
-econstructor. exact H. exact H0. easy.
-intros. specialize (H2 v).
-split. easy.
-apply LE. easy.
-econstructor. exact H. easy.
-apply LE. easy.
-Qed.
-Hint Resolve safe_monotone : paco.
-
-CoFixpoint paco_eqv_help {E F A} {VE : Spec E} {VF : Spec F} (i : ThreadName) (R G : Relt VE VF) (Q : Post VE VF A) (P : Relt VE VF) (C : Prog E A):
-  paco_safe i R G P C Q -> SafeProg i R G P C Q.
-intros.
-punfold H.
-dependent destruction H.
-econstructor. easy.
-econstructor. exact H. exact H0. easy.
-intros. specialize (H2 v). destruct_all.
-split. easy.
-destruct H3.
-apply paco_eqv_help. easy.
-destruct H3.
-destruct H1.
-econstructor. exact H. easy.
-apply paco_eqv_help. easy.
-destruct H1.
-Qed.
-
-Lemma paco_eqv {E F A} {VE : Spec E} {VF : Spec F} (i : ThreadName) (R G : Relt VE VF) (Q : Post VE VF A) (P : Relt VE VF) (C : Prog E A):
-  SafeProg i R G P C Q = paco_safe i R G P C Q.
-apply propositional_extensionality.
-split; intros.
-{
-  generalize dependent C. generalize dependent P.
-  pcofix rec. intros. pfold.
-  destruct H0.
-  econstructor. easy.
-  econstructor. exact H. exact H0. easy.
-  intros. specialize (H2 v). destruct_all.
-  split. easy.
-  right. apply rec. easy.
-  econstructor. exact H. easy.
-  right. apply rec. easy.
-}
-apply paco_eqv_help. easy.
-Qed.
 
 Section rules.
 
